Show that $x^ay^b$ is an integrating factor for the following equation and then find its solution.
\begin{equation*}
	(b+1)x\frac{dy}{dx}+(a+1)y=0
\end{equation*}

Begin by multiplying the entire equation by the integrating factor:

\begin{equation*}
	(b+1)x^{a+1}y^bdy+(a+1)x^ay^{b+1}dx=0
\end{equation*}

This can be seen to be in the form of an exact equation, with $M=(a+1)x^ay^{b+1}$ and $N=(b+1)x^{a+1}y^b$. Thus differentiating $M$ with respect to $y$ and $N$ with respect to $x$.
\begin{align*} 
b(a+1)x^ay^b &+(a+1)x^ay^b \\ 
a(b+1)x^ay^b &+(b+1)x^ay^b 
\end{align*}

As such, the integrating factor applies if and only if $a=b$. 

Begin by integrating $M$ with respect to $x$. $u(x,y)=\frac{ax^{a+1}}{a+1}y^{b+1}+\frac{x^{a+1}y^{b+1}}{a+1}+p(y)$. Differentiating this and setting equal to $N$ yields that $p(y)=0$. Thus combining yields:
\begin{equation*}
	\boxed{
	F(x,y)=\frac{ax^{a+1}}{a+1}y^{b+1}+\frac{x^{a+1}y^{b+1}}{a+1}+C}
\end{equation*}

