Find the solution of 
\begin{enumerate}
	\item $y\prime(x)=x(4-y)$
	\item $y\prime(x)+6x^2y=e^{-2x^3}/x^2$ with $y(1)=0$
\end{enumerate}

\begin{enumerate}
	\item By seperating variables, this quickly becomes $dy(4-y)^{-1}=xdx$. By integrating both sides, this becomes $-ln(4-y)=\frac{x^2}{2}+C_1$. Solving for $y$ explicitly this yields:
	\begin{equation*}
	\boxed{
		y=C_2-e^{-x^2/2}
		}
	\end{equation*}
	
	\item This is a first order, linear differential equation, as such the integrating factor is $q(x)=exp(\int 6x^2dx)=exp(2x^3)$. Thus multipling and integrating yields:
	\begin{equation*}
		y(x)=\frac{C}{e^{2x^3}}-\frac{1}{xe^{2x^3}}
	\end{equation*}
	After applying the boundary condition of $y(1)=0$:
	\begin{equation*}
	\boxed{
		y(x)=\frac{1}{e^{2x^3}}-\frac{1}{xe^{2x^3}}}
	\end{equation*}
\end{enumerate}
